powerpc/ConstpropOpproof.v
@@ -49,7 +49,7 @@ Hypothesis MATCH: ematch bc rs ae.
 
 Lemma match_G:
   forall r id ofs,
-  AE.get r ae = Ptr(Gl id ofs) -> Val.lessdef rs#r (symbol_address ge id ofs).
+  AE.get r ae = Ptr(Gl id ofs) -> Val.lessdef rs#r (Genv.symbol_address ge id ofs).
 Proof.
   intros. apply vmatch_ptr_gl with bc; auto. rewrite <- H. apply MATCH. 
 Qed.
@@ -82,7 +82,7 @@ Ltac SimplVM :=
       rewrite E in *; clear H; SimplVM
   | [ H: vmatch _ ?v (Ptr(Gl ?id ?ofs)) |- _ ] =>
       let E := fresh in
-      assert (E: Val.lessdef v (Op.symbol_address ge id ofs)) by (eapply vmatch_ptr_gl; eauto); 
+      assert (E: Val.lessdef v (Genv.symbol_address ge id ofs)) by (eapply vmatch_ptr_gl; eauto); 
       clear H; SimplVM
   | [ H: vmatch _ ?v (Ptr(Stk ?ofs)) |- _ ] =>
       let E := fresh in
@@ -436,13 +436,6 @@ Proof.
   exists v; auto.
 Qed.
 
-Remark shift_symbol_address:
-  forall symb ofs n,
-  Op.symbol_address ge symb (Int.add ofs n) = Val.add (Op.symbol_address ge symb ofs) (Vint n).
-Proof.
-  unfold Op.symbol_address; intros. destruct (Genv.find_symbol ge symb); auto. 
-Qed.
-
 Lemma addr_strength_reduction_correct:
   forall addr args vl res,
   vl = map (fun r => AE.get r ae) args ->
@@ -453,8 +446,8 @@ Proof.
   intros until res. unfold addr_strength_reduction.
   destruct (addr_strength_reduction_match addr args vl); simpl;
   intros VL EA; InvApproxRegs; SimplVM; try (inv EA).
-- rewrite shift_symbol_address. econstructor; split; eauto. apply Val.add_lessdef; auto. 
-- fold (Val.add (Vint n1) rs#r2). rewrite Int.add_commut. rewrite shift_symbol_address. rewrite Val.add_commut.
+- rewrite Genv.shift_symbol_address. econstructor; split; eauto. apply Val.add_lessdef; auto. 
+- fold (Val.add (Vint n1) rs#r2). rewrite Int.add_commut. rewrite Genv.shift_symbol_address. rewrite Val.add_commut.
   econstructor; split; eauto. apply Val.add_lessdef; auto.
 - rewrite Int.add_zero_l. 
   change (Vptr sp (Int.add n1 n2)) with (Val.add (Vptr sp n1) (Vint n2)).
@@ -467,8 +460,8 @@ Proof.
 - fold (Val.add (Vint n1) rs#r2).
   rewrite Val.add_commut. econstructor; split; eauto.
 - econstructor; split; eauto.
-- rewrite shift_symbol_address. econstructor; split; eauto. 
-- rewrite shift_symbol_address. econstructor; split; eauto. apply Val.add_lessdef; auto. 
+- rewrite Genv.shift_symbol_address. econstructor; split; eauto. 
+- rewrite Genv.shift_symbol_address. econstructor; split; eauto. apply Val.add_lessdef; auto. 
 - rewrite Int.add_zero_l.  
   change (Vptr sp (Int.add n1 n)) with (Val.add (Vptr sp n1) (Vint n)).
   econstructor; split; eauto. apply Val.add_lessdef; auto.
